src/NoVirtualMemory.v
@@ -1,0 +1,16 @@
+Require Import riscv.Program.
+Require Import riscv.util.Monad.
+Require Import riscv.util.NameWithEq.
+
+Inductive AccessType: Set := Instruction | Load | Store.
+
+Local Open Scope alu_scope.
+
+(* in a system with virtual memory, this would also do the translation, but in our
+   case, we only verify the alignment *)
+Definition withTranslation{N: NameWithEq}{t u: Set}{A: Alu t u}{M: Type -> Type}
+  {MM: Monad M}{RVS: RiscvState M}
+  (accessType: AccessType)(alignment: t)(addr: t)(memFunc: t -> M unit): M unit :=
+  if rem addr alignment /= zero
+  then raiseException zero four
+  else memFunc addr.
